---
sidebar_position: 13
---

# The Taylor Formula and Its Analytical Applications

## Definition of the $n$-th order taylor polynomial

Assume that $f$ has $n$ derivatives at $x_0$.  The $n$-th order Taylor polynomial of $f$ at $x_0$ is defined by

$$
\begin{equation*}
T_{f,x_0,n}(h)
= f(x_0)
+ f'(x_0) h
+ \frac{f''(x_0)}{2} h^2
+ \cdots
+ \frac{f^{(n)}(x_0)}{n!} h^n .
\end{equation*}
$$

We call $T_{f,x_0,n}(h)$ the **$n$-th order Taylor polynomial of $f$ at $x_0$**.



## Taylor’s theorem with peano remainder

If $f$ has $n$ derivatives at $x_0$, then a polynomial
$$
\begin{equation*}
P_n(h)=a_0+a_1 h+\cdots+a_n h^n
\end{equation*}
$$
satisfies
$$
\begin{equation*}
f(x_0+h)=P_n(h)+o(h^n),\qquad h\to 0,
\end{equation*}
$$
**if and only if** $P_n(h)$ is the $n$-th order Taylor polynomial of $f$ at $x_0$. ( Peano remainder )



## Taylor’s Theorem with lagrange remainder 

Assume that $f$ is continuous on an interval $I$ and $(n+1)$ times differentiable on the interior of $I$.  For any interior point $x_0\in I$ and any $x\in I$, there exists a point $\xi$ strictly between $x$ and $x_0$ such that

$$
\begin{equation*}
f(x)
= T_{f,x_0,n}(x - x_0)
+ \frac{f^{(n+1)}(\xi)}{(n+1)!}\,(x-x_0)^{\,n+1}.
\end{equation*}
$$

( Lagrange remainder )



## Examples

1. 

$$
\begin{equation*}
e^{x}
= 1 + x + \frac{x^{2}}{2}
+ \cdots + \frac{x^{n}}{n!}
+ o(x^{n}),\qquad x\to 0.
\end{equation*}
$$



2. 

3. $$
	\begin{equation*}
	\sin x
	= x - \frac{x^{3}}{3!}
	+ \cdots + (-1)^{n}\frac{x^{2n+1}}{(2n+1)!}
	+ o(x^{2n+2}),\qquad x\to 0,
	\end{equation*}
	$$



3. $$
	\begin{equation*}
	\cos x
	= 1 - \frac{x^{2}}{2!}
	+ \cdots + (-1)^{n}\frac{x^{2n}}{(2n)!}
	+ o(x^{2n+1}),\qquad x\to 0,
	\end{equation*}
	$$



4. $$
	\begin{equation*}
	\ln(1+x)
	= x- \frac{x^{2}}{2}
	+ \cdots + (-1)^{n-1}\frac{x^{n}}{n}
	+ o(x^{n}),\qquad x\to 0.
	\end{equation*}
	$$



5. $$
	\begin{equation*}
	(1+x)^{\alpha}
	= 1 + \alpha x
	+ \frac{\alpha(\alpha-1)}{2!}x^{2}
	+ \cdots
	+ \frac{\alpha(\alpha-1)\cdots(\alpha-n+1)}{n!}x^{n}
	+ o(x^{n}),\qquad x\to 0.
	\end{equation*}
	$$



6. 

7. $$
	\begin{equation*}
	\arctan x
	= x - \frac{x^{3}}{3}
	+ \cdots + (-1)^{n}\frac{x^{2n+1}}{2n+1}
	+ o(x^{2n + 2}),\qquad x\to 0,
	\end{equation*}
	$$



## Applications

1. Estimating the Error of Newton’s Method

Let $f(x^*) = 0$.  Define  
$$
\begin{equation*}
M = \max_{x\in[a,b]} |f''(x)|,\qquad
m = \min_{x\in[a,b]} |f'(x)|.
\end{equation*}
$$

Then the Newton iteration error satisfies:

Using the Newton iteration
$$
\begin{equation*}
x_{n+1} = x_n - \frac{f(x_n)}{f'(x_n)},
\end{equation*}
$$

we compute the error:

$$
\begin{equation*}
{x_{n+1} - x^*}
= x_n - x^* - \frac{f(x_n) - f(x^*)}{f'(x_n)}.
\end{equation*}
$$

Apply the Lagrange form of Taylor’s theorem:  for some $\xi$ strictly between $x_n$ and $x^*$,

$$
\begin{equation*}
f(x_n) - f(x^*) = f'(\xi)(x_n - x^*).
\end{equation*}
$$

Thus,
$$
\begin{equation*}
x_{n+1} - x^*
= (x_n - x^*)\left(1 - \frac{f'(\xi)}{f'(x_n)}\right).
\end{equation*}
$$



Using the mean value theorem again, for some $\eta$ between $x_n$ and $\xi$:
$$
\begin{equation*}
f'(\xi) = f'(x_n) + f''(\eta)(\xi - x_n).
\end{equation*}
$$

Substituting gives
$$
\begin{equation*}
x_{n+1} - x^*
= (x_n - x^*)
  \frac{f''(\eta)(x_n - \xi)}{f'(x_n)}.
\end{equation*}
$$



Taking absolute values:

$$
\begin{equation*}
|x_{n+1} - x^*|
\le \frac{M}{m}\, |x_n - x^*|^2.
\end{equation*}
$$

This shows the **quadratic convergence** of Newton’s method.
