---
sidebar_position: 14
---

# The Concept and Computation of Indefinite Integrals

## The concept of indefinite integrals

A function $F$ is called an **antiderivative** of a function $f$ on an interval $I \subset \mathbb{R}$ if  
$$
\begin{equation*}
F'(x) = f(x), \qquad \forall x \in I.
\end{equation*}
$$

The **indefinite integral** of $f$ on $I \subset \mathbb{R}$ is the **family of all antiderivatives** of $f$ on $I$, and is denoted by

$$
\begin{equation*}
\int f(x)\, dx.
\end{equation*}
$$


Let $I \subset \mathbb{R}$ be an interval.  If $F_1$ and $F_2$ are two antiderivatives of $f$ on $I$,  then the difference $F_1(x) - F_2(x)$ is a constant. Consequently,
$$
\begin{equation*}
\int f(x)\, dx = F(x) + C,
\end{equation*}
$$

where $F$ is any antiderivative of $f$ on $I$, and $C$ is an arbitrary constant.



### Examples

1. $$
	\begin{equation*}
	\int e^{x}\, dx = e^{x} + C.
	\end{equation*}
	$$

	



2. $$
	\begin{equation*}
	\int \sin x\, dx = -\cos x + C,
	\end{equation*}
	$$


$$
\begin{equation*}
\int \cos x\, dx = \sin x + C.
\end{equation*}
$$



3. 

$$
\begin{equation*}
\int \sinh x\, dx = \cosh x + C,
\end{equation*}
$$

$$
\begin{equation*}
\int \cosh x\, dx = \sinh x + C.
\end{equation*}
$$

Where
$$
\begin{equation*}
\sinh x = \frac{e^{x} - e^{-x}}{2},\qquad
\cosh x = \frac{e^{x} + e^{-x}}{2}.
\end{equation*}
$$


4. For $\alpha \ne -1$,
	$$
	\begin{equation*}
	\int x^{\alpha}\, dx
	= \frac{x^{\alpha+1}}{\alpha+1} + C.
	\end{equation*}
	$$



5. $$
	\begin{equation*}
	\int \frac{1}{x}\, dx = \ln|x| + C.
	\end{equation*}
	$$





6. $$
	\begin{equation*}
	\int \frac{1}{1+x^{2}}\, dx = \arctan x + C.
	\end{equation*}
	$$



### Theorems

1. If $F$ and $G$ are antiderivatives of $f$ and $g$ on an interval $I$,  then $\lambda F + \mu G$ is an antiderivative of $\lambda f + \mu g$ on $I$.  Consequently,
	$$
	\begin{equation*}
	\int \bigl(\lambda f(x) + \mu g(x)\bigr)\, dx
	= \lambda \int f(x)\, dx
	+ \mu \int g(x)\, dx.
	\end{equation*}
	$$



2. If $F$ and $G$ are antiderivatives of $f$ and $g$, respectively,  then
	$$
	\begin{equation*}
	\int f(G(x))\, g(x)\, dx
	= F(G(x)) + C.
	\end{equation*}
	$$



3. If $F$ and $G$ are antiderivatives of $f$ and $g$ on an interval $I$, then

	$$
	\begin{equation*}
	\int F(x)\, g(x)\, dx
	= F(x) G(x) - \int G(x)\, f(x)\, dx.
	\end{equation*}
	$$



## The computation of indefinite integrals

1. Compute
	$$
	\begin{equation*}
	\int \frac{x}{1+x^{2}}\, dx.
	\end{equation*}
	$$

	Let
	$$
	\begin{equation*}
	y = 1 + x^{2}, \qquad dy = 2x\, dx.
	\end{equation*}
	$$

	Then
	$$
	\begin{equation*}
	\int \frac{x}{1+x^{2}}\, dx
	= \frac{1}{2} \int \frac{1}{1+x^{2}}\, d(1+x^{2})
	= \frac{1}{2} \int \frac{1}{y}\, dy.
	\end{equation*}
	$$

	Thus
	$$
	\begin{equation*}
	\frac{1}{2}\int \frac{1}{y}\, dy
	= \frac{1}{2}\ln|y| + C
	= \frac{1}{2}\ln(1+x^{2}) + C.
	\end{equation*}
	$$



2. Compute
$$
\begin{equation*}
\int \frac{1}{\cos^{2m} x}\, dx.
\end{equation*}
$$

Let
$$
\begin{equation*}
t = \tan x, \qquad dt = \sec^{2}x\, dx = \frac{1}{\cos^{2}x}\, dx.
\end{equation*}
$$

Then
$$
\begin{equation*}
\int \frac{1}{\cos^{2m} x}\, dx
= \int \frac{1}{\cos^{2m-2} x}\, d(\tan x)
= \int (1+t^{2})^{\,m-1}\, dt.
\end{equation*}
$$

Thus the integral can be reduced to a polynomial-type integral in $t$:
$$
\begin{equation*}
\int \frac{1}{\cos^{2m} x}\, dx
= \int (1+t^{2})^{\,m-1}\, dt,
\qquad t=\tan x.
\end{equation*}
$$


3. Compute
$$
\begin{equation*}
\int f(\cos^{2} x)\, dx.
\end{equation*}
$$

We first rewrite the integrand:
$$
\begin{equation*}
\int f(\cos^{2} x)\, dx
= \int \frac{f(\cos^{2} x)\,\cos^{2}x}{\cos^{2}x}\, dx.
\end{equation*}
$$

Let
$$
\begin{equation*}
t = \tan x, \qquad dt = \frac{1}{\cos^{2}x}\, dx, \qquad
\cos^{2}x = \frac{1}{1+t^{2}}.
\end{equation*}
$$

Then
$$
\begin{equation*}
\int f(\cos^{2} x)\, dx
= \int \frac{1}{1+t^{2}}\, f\!\left(\frac{1}{1+t^{2}}\right)\, dt.
\end{equation*}
$$

Thus the integral of $f(\cos^{2}x)$ is transformed into an integral in $t$:
$$
\begin{equation*}
\int f(\cos^{2} x)\, dx
= \int \frac{1}{1+t^{2}}\, f\!\left(\frac{1}{1+t^{2}}\right)\, dt,
\qquad t=\tan x.
\end{equation*}
$$


4. Compute
	$$
	\begin{equation*}
	\int \frac{1}{\sqrt{x^{2}+a^{2}}}\, dx
	\end{equation*}
	$$

	Let
	$$
	\begin{equation*}
	\theta = \arctan\!\left(\frac{x}{a}\right)
	\end{equation*}
	$$

	Then
	$$
	\begin{equation*}
	\int \frac{1}{\sqrt{x^{2}+a^{2}}}\, dx
	= \int \frac{1}{\sqrt{a^{2}\tan^{2}\theta + a^{2}}}\, d(a\tan\theta)
	\end{equation*}
	$$

	Since
	$$
	\begin{equation*}
	\sqrt{a^{2}\tan^{2}\theta + a^{2}}
	= a\sqrt{1+\tan^{2}\theta}
	= \frac{a}{\cos\theta},
	\end{equation*}
	$$

	we have
	$$
	\begin{equation*}
	\int \frac{1}{\sqrt{x^{2}+a^{2}}}\, dx
	= \int \frac{1}{\cos\theta}\, d\theta
	\end{equation*}
	$$

	Let
	$$
	\begin{equation*}
	t = \sin\theta,
	\qquad dt = \cos\theta\, d\theta .
	\end{equation*}
	$$

	Then
	$$
	\begin{equation*}
	\int \frac{1}{\cos\theta}\, d\theta
	= \frac{1}{2}\int \left(\frac{1}{1-t} + \frac{1}{1+t}\right) dt
	= \frac{1}{2}\ln\frac{1+t}{1-t} + C
	\end{equation*}
	$$

	Thus
	$$
	\begin{equation*}
	\frac{1}{2}\ln\frac{1+\sin\theta}{1-\sin\theta} + C
	\end{equation*}
	$$

	Since
	$$
	\begin{equation*}
	\sin\theta = \frac{x}{\sqrt{a^{2}+x^{2}}},
	\end{equation*}
	$$

	we get
	$$
	\begin{equation*}
	\frac{1}{2}\ln
	\left(
	\frac{1+\frac{x}{\sqrt{a^{2}+x^{2}}}}
	     {1-\frac{x}{\sqrt{a^{2}+x^{2}}}}
	\right)
	= \ln\left(x+\sqrt{a^{2}+x^{2}}\right) + C_1.
	\end{equation*}
	$$

	Therefore
	$$
	\begin{equation*}
	\int \frac{1}{\sqrt{x^{2}+a^{2}}}\, dx
	= \ln\left(x+\sqrt{a^{2}+x^{2}}\right) + C .
	\end{equation*}
	$$



5. Let
	$$
	\begin{equation*}
	I_n = \int e^{x}\sin^{n}x\, dx .
	\end{equation*}
	$$

	Then
	$$
	\begin{equation*}
	I_n = \int e^{x}\sin^{n}x\, dx
	= \int \sin^{n}x\, d(e^{x})
	= e^{x}\sin^{n}x - \int e^{x} d(\sin^{n}x).
	\end{equation*}
	$$

	Compute the differential:
	$$
	\begin{equation*}
	d(\sin^{n}x)
	= n\sin^{\,n-1}x \cos x\, dx.
	\end{equation*}
	$$

	Hence
	$$
	\begin{equation*}
	I_n
	= e^{x}\sin^{n}x - n\int \sin^{\,n-1}x \cos x\, e^{x}\, dx.
	\end{equation*}
	$$

	Rewrite the integral:
	$$
	\begin{equation*}
	I_n
	= e^{x}\sin^{n}x - n e^{x}\sin^{\,n-1}x\cos x
	+ n\int e^{x} d(\sin^{\,n-1}x\cos x).
	\end{equation*}
	$$

	Thus
	$$
	\begin{equation*}
	I_n
	= e^{x}\bigl(\sin^{n}x - n\sin^{\,n-1}x\cos x\bigr)
	+ n(n-1)(I_{n-2} - I_n) - n I_n .
	\end{equation*}
	$$

	Solve for \(I_n\):
	$$
	\begin{equation*}
	I_n
	= \frac{
	e^{x}\sin^{\,n-1}x\bigl(\sin x - n\cos x\bigr)
	+ n(n-1)I_{n-2}
	}{n^{2}+1}.
	\end{equation*}
	$$

	Special case:
	$$
	\begin{equation*}
	I_1 = \frac{e^{x}(\sin x - \cos x)}{2}.
	\end{equation*}
	$$



6. A **rational function** is a quotient of two polynomials:

	$$
	\begin{equation*}
	R(x)=\frac{P(x)}{Q(x)}, \qquad P, Q \in \mathbb{R}[x], \quad Q(x)\neq 0.
	\end{equation*}
	$$

	To integrate $R(x)$, follow these steps.

​	**Polynomial Long Division**

​	If  
$$
\begin{equation*}
\deg P \ge \deg Q,
\end{equation*}
$$
​	divide $P$ by $Q$:
$$
\begin{equation*}
\frac{P(x)}{Q(x)} = S(x) + \frac{A(x)}{Q(x)}, 
\qquad \deg A < \deg Q.
\end{equation*}
$$
​	Thus,
$$
\begin{equation*}
\int R(x)\,dx = \int S(x)\,dx + \int \frac{A(x)}{Q(x)}\, dx.
\end{equation*}
$$


​	**Factor the Denominator**

​	Factor $Q(x)$ into irreducible real factors:

$$
\begin{equation*}
Q(x)=
\prod (x-a_i)^{k_i}
\prod (x^2 + b_j x + c_j)^{m_j},
\end{equation*}
$$

​	where each quadratic satisfies  
$$
\begin{equation*}
b_j^2 - 4c_j < 0.
\end{equation*}
$$
​	

​	**Partial Fraction Decomposition**
$$
\begin{equation*}
\frac{A_1}{x-a} + \frac{A_2}{(x-a)^2} + \cdots + \frac{A_k}{(x-a)^k}
\end{equation*}
$$

$$
\begin{equation*}
\frac{A_1x+B_1}{x^2+bx+c}
+ \frac{A_2x+B_2}{(x^2+bx+c)^2}
+ \cdots +
\frac{A_mx+B_m}{(x^2+bx+c)^m}.
\end{equation*}
$$



​	**Integrate Each Term**
$$
\begin{equation*}
\int \frac{1}{x-a}\, dx = \ln |x-a| + C.
\end{equation*}
$$

$$
\begin{equation*}
\int \frac{1}{(x-a)^k}\, dx 
= \frac{-(x-a)^{-k+1}}{k-1} + C \qquad (k\ge 2).
\end{equation*}
$$

$$
\begin{equation*}
x^2+bx+c = \left(x+\frac{b}{2}\right)^2 + d, \quad d = c-\frac{b^2}{4}.
\end{equation*}
$$

$$
\begin{equation*}
\int \frac{1}{(x+\frac{b}{2})^2+d}\, dx
= \frac{1}{\sqrt{d}} \arctan\!\left(\frac{x+\frac{b}{2}}{\sqrt{d}}\right) + C.
\end{equation*}
$$

$$
\begin{equation*}
\int \frac{x+\frac{b}{2}}{(x+\frac{b}{2})^2+d}\, dx
= \frac{1}{2}\ln\left((x+\frac{b}{2})^2+d\right) + C.
\end{equation*}
$$



​	

6. $$
	\begin{equation*}
	I_n = \int \frac{1}{(1+x^2)^n}\,dx
	\qquad (n\ge 2).
	\end{equation*}
	$$

	Write

	$$
	\begin{equation*}
	I_n = \int \frac{1}{(1+x^2)^n}\,dx
	= \int \frac{(1+x^2)-x^2}{(1+x^2)^n}\,dx
	= I_{n - 1}
	     - \int \frac{x^2}{(1+x^2)^n}\,dx.
	\end{equation*}
	$$
	
	
	
	$$
	\begin{equation*}
	\begin{aligned}
	&\int \frac{x^2}{(1+x^2)^n}\,dx
	= \frac{1}{2}\int \frac{x}{(1+x^2)^{n}} \,d(1 + x^2)
	= \frac{1}{2 (1 - n)}\int x \,d\left((1 + x^2) ^ {1 - n}\right) \\
	&= \frac{1}{2 (1 - n)} \left( \frac{x}{(1+x^2)^{n-1}} - \int \frac{1}{(1 + x^2)^{n - 1}} \, dx\right).
	\end{aligned}
	\end{equation*}
	$$
	
	Therefore
	
	$$
	\begin{equation*}
	I_n
	= \left(1 - \frac{1}{2(n-1)}\right) I_{n-1}
	  + \frac{1}{2(n-1)}\frac{x}{(1+x^2)^{n-1}}.
	\end{equation*}
	$$
	
	
	
	Thus the **reduction formula** is
	$$
	\begin{equation*}
	I_n
	= \frac{x}{2(n-1)(1+x^2)^{n-1}}
	+ \frac{2n-3}{2(n-1)}\, I_{n-1},
	\qquad n\ge 2.
	\end{equation*}
	$$
	
	Together with
	
	$$
	\begin{equation*}
	I_1 = \int \frac{dx}{1+x^2} = \arctan x + C,
	\end{equation*}
	$$





7. $$
	\begin{equation*}
	\int R(\cos\theta,\sin\theta)\, d\theta
	=
	\int 
	R\!\left(
	\frac{1 - t^{2}}{1 + t^{2}},\;
	\frac{2t}{1 + t^{2}}
	\right)
	\frac{2}{1+t^{2}}\, dt.
	\end{equation*}
	$$


$$
\begin{equation*}
\int R(x,\sqrt{x^{2}-1})\, dx
=
\int 
R\!\left(
\frac{1+t^{2}}{1-t^{2}},\;
\frac{2t}{\,1-t^{2}\,}
\right)
\, d\!\left(\frac{1+t^{2}}{1-t^{2}}\right).
\end{equation*}
$$
